Cleaned up exception handing example

examples/dm4all/ExnHandle.fst
@@ -48,7 +48,7 @@ effect Exn (a:Type) (pre:Type0) (post:either a exn -> Type0) =
 val raise : #a:Type0 -> e:exn -> EXN a (fun p -> p (Inr e))
 let raise #a e = EXN?.reflect (Inr e)
 
-(* The algebra extension operation is inlined for better readability *)
+(* The algebra extension operation (h_c)_* is inlined for better readability *)
 
 let handle_rep (#a:Type) 
                (#b:Type)
@@ -58,59 +58,6 @@ let handle_rep (#a:Type)
   match c1 with
   | Inl x -> c2 x
   | Inr e -> h_c e
-
-unfold
-let handle_wp (#a:Type) 
-              (#b:Type) 
-              (wp1:wp_type a) 
-              (h_wp:exn -> wp_type b) 
-              (wp2:a -> wp_type b) : wp_type b = 
-  fun p -> wp1 (fun r -> match r with
-                         | Inl x -> wp2 x p
-                         | Inr e -> h_wp e p)
-
-let lemma_handle (#a:Type) 
-                 (#b:Type) 
-                 (wp1:wp_type a)
-                 (c1:either a exn)
-                 (h_wp:exn -> wp_type b) 
-                 (h_c:(e:exn -> either b exn))
-                 (wp2:a -> wp_type b) 
-                 (c2:(x:a -> either b exn))
-  : Lemma (requires ((forall p . wp1 p ==> p c1) /\
-                     (forall p x . wp2 x p ==> p (c2 x)) /\ 
-                     (forall p e . h_wp e p ==> p (h_c e))))
-          (ensures  (forall p . 
-                     wp1 (fun r -> (match r with | Inl x -> wp2 x p | Inr e -> h_wp e p)) 
-                     ==>
-                     p (match c1 with | Inl x -> c2 x | Inr e -> h_c e))) =
-  match c1 with
-  | Inl x -> ()
-  | Inr e -> ()
-
-let related #a (r : repr a) (wp : wp_type a) =
-  EXN?.stronger _ wp (interp _ r)
-
-(* We should get this from the framework FIXME *)
-assume val reify_related (#a #b:Type) (wp:_) (c : (x:a -> EXN b (wp x))) :
-                         Lemma (forall (x:a). related (reify (c x)) (wp x))
-
-let catch (#a:Type) 
-           (#b:Type) 
-           (#wp1:wp_type a) 
-           (c1:unit -> EXN a wp1)
-           (#h_wp:exn -> wp_type b) 
-           (h_c:(e:exn -> EXN b (h_wp e)))
-           (#wp2:a -> wp_type b) 
-           (c2:(x:a -> EXN b (wp2 x))) 
-         : EXN b (handle_wp wp1 h_wp wp2) =
-  reify_related (fun _ -> wp1) c1;
-  reify_related wp2 c2;
-  reify_related h_wp h_c;
-  lemma_handle wp1 (reify (c1 ())) (h_wp) (fun e -> reify (h_c e)) wp2 (fun x -> reify (c2 x));
-  EXN?.reflect (handle_rep (reify (c1 ()) <: either a exn) 
-                           (fun e -> reify (h_c e)) 
-                           (fun x -> reify (c2 x)))
 
 unfold
 let wp_return (#a:Type) (x:a) : wp_type a = fun p -> p (Inl x)
@@ -124,6 +71,54 @@ let wp_bind (#a:Type) (#b:Type) (wp : wp_type a) (f : a -> wp_type b) =
 unfold
 let wp_raise (#a:Type) (e:exn) : wp_type a = fun p -> p (Inr e)
 
+unfold
+let wp_try_catch (#a:Type) 
+                 (#b:Type) 
+                 (wp1:wp_type a) 
+                 (h_wp:exn -> wp_type b) 
+                 (wp2:a -> wp_type b) : wp_type b = 
+  fun p -> wp1 (fun r -> match r with
+                         | Inl x -> wp2 x p
+                         | Inr e -> h_wp e p)
+
+let related #a (r : repr a) (wp : wp_type a) =
+  EXN?.stronger _ wp (interp _ r)
+
+(* We should get this from the framework FIXME *)
+assume val reify_related (#a #b:Type) (wp:_) (c : (x:a -> EXN b (wp x))) :
+                         Lemma (forall (x:a). related (reify (c x)) (wp x))
+
+let lemma_try_catch (#a:Type) 
+                    (#b:Type) 
+                    (wp1:wp_type a)
+                    (c1:either a exn)
+                    (h_wp:exn -> wp_type b) 
+                    (h_c:(e:exn -> either b exn))
+                    (wp2:a -> wp_type b) 
+                    (c2:(x:a -> either b exn))
+  : Lemma (requires ((related c1 wp1) /\
+                     (forall x . related (c2 x) (wp2 x)) /\ 
+                     (forall e . related (h_c e) (h_wp e))))
+          (ensures  (related (handle_rep c1 h_c c2) (wp_try_catch wp1 h_wp wp2))) =
+  match c1 with
+  | Inl x -> ()
+  | Inr e -> ()
+
+let try_catch (#a:Type) 
+              (#b:Type) 
+              (#wp1:wp_type a) 
+              (c1:unit -> EXN a wp1)
+              (#h_wp:exn -> wp_type b) 
+              (h_c:(e:exn -> EXN b (h_wp e)))
+              (#wp2:a -> wp_type b) 
+              (c2:(x:a -> EXN b (wp2 x))) 
+            : EXN b (wp_try_catch wp1 h_wp wp2) =
+  reify_related (fun _ -> wp1) c1;
+  reify_related wp2 c2;
+  reify_related h_wp h_c;
+  lemma_try_catch wp1 (reify (c1 ())) (h_wp) (fun e -> reify (h_c e)) wp2 (fun x -> reify (c2 x));
+  EXN?.reflect (handle_rep (reify (c1 ())) (fun e -> reify (h_c e)) (fun x -> reify (c2 x)))
+
 let test1 (#a:Type) 
           (#b:Type) 
           (#wp1:wp_type a) 
@@ -131,7 +126,7 @@ let test1 (#a:Type)
           (#wp2:a -> wp_type b) 
           (c2:(x:a -> EXN b (wp2 x))) 
         : EXN b (wp_bind wp1 wp2) =
-  catch #a #b #wp1 c1 #(fun e -> wp_raise e) (fun e -> raise e) #wp2 c2
+  try_catch #_ #_ #wp1 c1 #(fun e -> wp_raise e) (fun e -> raise e) #wp2 c2
 
 let test2 (#a:Type) 
           (#b:Type) 
@@ -141,7 +136,7 @@ let test2 (#a:Type)
           (#wp2:a -> wp_type b) 
           (c2:(x:a -> EXN b (wp2 x))) 
         : EXN b (wp2 v) = 
-  catch #a #b #(wp_return v) (fun _ -> v) #h_wp h_c #wp2 c2
+  try_catch #_ #_ #(wp_return v) (fun _ -> v) #h_wp h_c #wp2 c2
 
 let test3 (#a:Type) 
           (#b:Type) 
@@ -151,7 +146,7 @@ let test3 (#a:Type)
           (#wp2:a -> wp_type b) 
           (c2:(x:a -> EXN b (wp2 x)))
         : EXN b (h_wp e) =
-  catch #a #b #(wp_raise e) (fun _ -> raise e) #h_wp h_c #wp2 c2
+  try_catch #_ #_ #(wp_raise e) (fun _ -> raise e) #h_wp h_c #wp2 c2
 
 assume val div_exn : exn
 
@@ -168,4 +163,4 @@ let div (i j:int)
 
 let try_div (i j:int)
   : EXN int (fun p -> forall x . Inl? x ==> p x) =
-  catch #int #int #(div_wp i j) (fun _ -> div i j) #(fun _ p -> p (Inl 0)) (fun _ -> 0) #(wp_return) (fun x -> x)
+  try_catch #_ #_ #(div_wp i j) (fun _ -> div i j) #(fun _ -> wp_return 0) (fun _ -> 0) #(wp_return) (fun x -> x)
